cedar-lean/Cedar/Thm/Validation/Levels/Basic.lean
@@ -14,11 +14,6 @@
  limitations under the License.
 -/
 
-import Cedar.Spec
-import Cedar.Data
-import Cedar.Validation
-import Cedar.Thm.Validation.Typechecker
-import Cedar.Thm.Validation.Typechecker.Types
 import Cedar.Thm.Validation.Typechecker.Basic
 
 namespace Cedar.Thm
@@ -27,7 +22,6 @@ namespace Cedar.Thm
 Basic definitions for levels proof
 -/
 
-open Cedar.Data
 open Cedar.Spec
 open Cedar.Validation
 
